pause proof with wire

NLustre/NLSemanticsCoIndWire.v
@@ -2,6 +2,7 @@ Require Import List.
 Import List.ListNotations.
 Open Scope list_scope.
 Require Import Coq.Sorting.Permutation.
+Require Import Setoid.
 
 Require Import Coq.FSets.FMapPositive.
 Require Import Velus.Common.
@@ -10,7 +11,7 @@ Require Import Velus.Clocks.
 Require Import Velus.NLustre.NLSyntax.
 Require Import Velus.NLustre.NLSemanticsCommon.
 Require Import Velus.NLustre.Ordered.
-Require Import Streams.
+Require Import Velus.NLustre.Streams.
 
 (** * The NLustre semantics *)
 
@@ -30,18 +31,17 @@ Module Type NLSEMANTICSCOINDWIRE
        (Import Comm  : NLSEMANTICSCOMMON Ids Op OpAux Clks Syn)
        (Import Ord   : ORDERED   Ids Op Clks Syn).
 
-  CoFixpoint fby1 (rs: Stream bool) (v c: val) (xs: Stream value) : Stream value :=
-    match rs, xs with
-    | false ::: rs, absent ::: xs => absent ::: fby1 rs v c xs
-    | true ::: rs, absent ::: xs => absent ::: fby rs c xs
-    | false ::: rs, present x ::: xs => present v ::: fby1 rs x c xs
-    | true ::: rs, present x ::: xs => present c ::: fby1 rs x c xs
+  CoFixpoint fby (rs: Stream bool) (c: val) (xs: Stream value) : Stream value :=
+    match xs with
+    | absent ::: xs => absent ::: fby (tl rs) c xs
+    | present x ::: xs => present c ::: fby1 (tl rs) x c xs
     end
-
-  with fby (rs: Stream bool) (c: val) (xs: Stream value) : Stream value :=
-         match xs with
-         | absent ::: xs => absent ::: fby (tl rs) c xs
-         | present x ::: xs => present c ::: fby1 (tl rs) x c xs
+  with fby1 (rs: Stream bool) (v c: val) (xs: Stream value) : Stream value :=
+         match rs, xs with
+         | false ::: rs, absent ::: xs => absent ::: fby1 rs v c xs
+         | true ::: rs, absent ::: xs => absent ::: fby rs c xs
+         | false ::: rs, present x ::: xs => present v ::: fby1 rs x c xs
+         | true ::: rs, present x ::: xs => present c ::: fby1 rs x c xs
          end.
 
   (* CoInductive fby1 *)
@@ -183,6 +183,97 @@ Module Type NLSEMANTICSCOINDWIRE
     Combined Scheme sem_equation_node_ind from sem_equation_mult, sem_node_mult.
 
   End SemInd.
+
+  Add Parametric Morphism : merge_reset
+      with signature @EqSt bool ==> @EqSt bool ==> @EqSt bool
+        as merge_reset_EqSt.
+  Proof.
+    cofix Cofix.
+    intros r1 r1' Er1 r2 r2' Er2.
+    unfold_St r1; unfold_St r1'; unfold_St r2; unfold_St r2'.
+    constructor; inv Er1; inv Er2; simpl in *; auto.
+    now subst.
+  Qed.
+
+  CoFixpoint wire_fby1_EqSt_fix (v c: val)
+           (rs rs': Stream bool) (Ers: rs ≡ rs')
+           (xs xs': Stream value) (Exs: xs ≡ xs') :
+    fby1 rs v c xs ≡ fby1 rs' v c xs'
+  with wire_fby_EqSt_fix (c: val)
+                     (rs rs': Stream bool) (Ers: rs ≡ rs')
+                     (xs xs': Stream value) (Exs: xs ≡ xs') :
+         fby rs c xs ≡ fby rs' c xs'.
+  Proof.
+    - unfold_Stv rs; unfold_Stv rs'; unfold_Stv xs; unfold_Stv xs';
+        constructor; inv Exs; inv Ers; simpl in *; try discriminate; auto.
+      + inv H; apply wire_fby1_EqSt_fix; auto.
+      + inv H; apply wire_fby1_EqSt_fix; auto.
+    - unfold_Stv xs; unfold_Stv xs'; unfold_St rs; unfold_St rs';
+        constructor; inv Exs; inv Ers; simpl in *; try discriminate; auto.
+      inv H; apply wire_fby1_EqSt_fix; auto.
+  Qed.
+
+  Add Parametric Morphism : fby
+      with signature @EqSt bool ==> eq ==> @EqSt value ==> @EqSt value
+        as wire_fby_EqSt.
+  Proof. intros; apply wire_fby_EqSt_fix; auto. Qed.
+
+  Fixpoint wire_sem_equation_morph_fix
+           (G: global) (H: history)
+           (b b': Stream bool) (Eb: b ≡ b')
+           (r r': Stream bool) (Er: r ≡ r')
+           (e: equation)
+           (Sem: sem_equation G H b r e) {struct Sem} :
+    sem_equation G H b' r' e
+  with wire_sem_node_morph_fix
+         (G: global)
+         (r r': Stream bool) (Er: r ≡ r')
+         (f: ident)
+         (xss xss': list (Stream value)) (Exss: EqSts value xss xss')
+         (yss yss': list (Stream value)) (Eyss: EqSts value yss yss')
+         (Sem: sem_node G r f xss yss) {struct Sem} :
+    sem_node G r' f xss' yss'.
+  Proof.
+    - induction Sem.
+      + econstructor; eauto.
+        now rewrite <-Eb.
+      + econstructor; eauto.
+        * apply Forall2_impl_In with (P:=sem_lexp H b); eauto.
+          intros; now rewrite <-Eb.
+        * eapply wire_sem_node_morph_fix; eauto; reflexivity.
+      + econstructor; eauto.
+        * apply Forall2_impl_In with (P:=sem_lexp H b); eauto.
+          intros; now rewrite <-Eb.
+        * eapply wire_sem_node_morph_fix; eauto; try reflexivity.
+          rewrite <-Er; reflexivity.
+      + econstructor; eauto.
+        * rewrite <-Eb; eauto.
+        * subst.
+          eapply sem_var_EqSt; eauto.
+          now rewrite <-Er.
+    - induction Sem.
+      econstructor; eauto.
+      + instantiate (1:=H).
+        now rewrite <-Exss.
+      + now rewrite <-Eyss.
+      + apply Forall_impl with (P:=sem_equation G H (clocks_of xss) r); auto.
+        apply wire_sem_equation_morph_fix; auto.
+        now rewrite Exss.
+  Admitted.
+
+  Add Parametric Morphism G H : (sem_equation G H)
+      with signature @EqSt bool ==> @EqSt bool ==> eq ==> Basics.impl
+        as wire_sem_equation_morph.
+  Proof.
+    unfold Basics.impl; apply wire_sem_equation_morph_fix.
+  Qed.
+
+  Add Parametric Morphism G : (sem_node G)
+      with signature @EqSt bool ==> eq ==> @EqSts value ==> @EqSts value ==> Basics.impl
+        as wire_sem_node_morph.
+  Proof.
+    unfold Basics.impl; apply wire_sem_node_morph_fix.
+  Qed.
 
 End NLSEMANTICSCOINDWIRE.
 
