NLustre/SemEquiv.v
@@ -26,372 +26,7 @@ Module Type SEMEQUIV
        (Import Comm  : NLSEMANTICSCOMMON Ids Op OpAux Clks Syn)
        (Import Ord   : ORDERED   Ids Op Clks Syn)
        (Wire         : NLSEMANTICSCOINDWIRE Ids Op OpAux Clks Syn Comm Ord)
-       (Rec          : NLSEMANTICSCOIND Ids Op OpAux Clks Syn Comm Ord).
-
-   Ltac unfold_Stv xs :=
-    rewrite (unfold_Stream xs);
-    destruct xs as [[|]];
-    simpl.
-
-  Ltac unfold_St xs :=
-    rewrite (unfold_Stream xs);
-    destruct xs;
-    simpl.
-
-  Add Parametric Relation A : (Stream A) (@EqSt A)
-      reflexivity proved by (@EqSt_reflex A)
-      symmetry proved by (@sym_EqSt A)
-      transitivity proved by (@trans_EqSt A)
-        as EqStrel.
-
-  Add Parametric Morphism A : (@Cons A)
-      with signature eq ==> @EqSt A ==> @EqSt A
-        as Cons_EqSt.
-  Proof.
-    cofix Cofix.
-    intros x xs xs' Exs.
-    constructor; simpl; auto.
-  Qed.
-
-  Add Parametric Morphism A : (@hd A)
-      with signature @EqSt A ==> eq
-        as hd_EqSt.
-  Proof.
-    intros xs xs' Exs.
-    destruct xs, xs'; inv Exs; simpl; auto.
-  Qed.
-
-  Add Parametric Morphism A : (@tl A)
-      with signature @EqSt A ==> @EqSt A
-        as tl_EqSt.
-  Proof.
-    intros xs xs' Exs.
-    destruct xs, xs'; inv Exs; simpl; auto.
-  Qed.
-
-  Section EqSts.
-    Variable A: Type.
-
-    Definition EqSts (xss yss: list (Stream A)) :=
-      Forall2 (@EqSt A) xss yss.
-
-    Theorem EqSts_reflex: forall xss, EqSts xss xss.
-    Proof.
-      induction xss; constructor; auto.
-      reflexivity.
-    Qed.
-
-    Theorem EqSts_sym: forall xss yss, EqSts xss yss -> EqSts yss xss.
-    Proof.
-      induction xss, yss; intros ** H; auto; try inv H.
-      constructor.
-      - now symmetry.
-      - now apply IHxss.
-    Qed.
-
-    Theorem EqSts_trans: forall xss yss zss, EqSts xss yss -> EqSts yss zss -> EqSts xss zss.
-    Proof.
-      induction xss, yss, zss; intros ** Hx Hy; auto; try inv Hx; try inv Hy.
-      constructor.
-      - now transitivity s.
-      - eapply IHxss; eauto.
-    Qed.
-
-  End EqSts.
-
-  Add Parametric Relation A : (list (Stream A)) (@EqSts A)
-      reflexivity proved by (@EqSts_reflex A)
-      symmetry proved by (@EqSts_sym A)
-      transitivity proved by (@EqSts_trans A)
-        as EqStsrel.
-
-  Add Parametric Morphism A : (@cons (Stream A))
-      with signature @EqSt A ==> @EqSts A ==> @EqSts A
-        as cons_EqSt.
-  Proof. constructor; auto. Qed.
-
-  Add Parametric Morphism
-      A B (P: A -> Stream B -> Prop) xs
-      (P_compat: Proper (eq ==> @EqSt B ==> Basics.impl) P)
-    : (@Forall2 A (Stream B) P xs)
-      with signature @EqSts B ==> Basics.impl
-        as Forall2_EqSt.
-  Proof.
-    intros ys ys' Eys.
-    revert xs ys ys' Eys;
-      induction xs, ys; intros ** H; inv H; inv Eys; auto.
-    constructor; eauto.
-    - eapply P_compat; eauto.
-    - eapply IHxs; eauto.
-  Qed.
-
-  Remark MapsTo_sem_var:
-    forall H x xs,
-      PM.MapsTo x xs H ->
-      sem_var H x xs.
-  Proof.
-    econstructor; eauto; reflexivity.
-  Qed.
-
-  Add Parametric Morphism H : (sem_var H)
-      with signature eq ==> @EqSt value ==> Basics.impl
-        as sem_var_EqSt.
-  Proof.
-    intros x xs xs' E.
-    intros Sem; induction Sem.
-    econstructor; eauto.
-    transitivity xs; auto; symmetry; auto.
-  Qed.
-
-  Add Parametric Morphism : merge
-      with signature @EqSt value ==> @EqSt value ==> @EqSt value ==> @EqSt value ==> Basics.impl
-        as merge_EqSt.
-  Proof.
-    cofix Cofix.
-    intros cs cs' Ecs xs xs' Exs ys ys' Eys zs zs' Ezs H.
-    destruct cs' as [[]], xs' as [[]], ys' as [[]], zs' as [[]];
-      inv H; inv Ecs; inv Exs; inv Eys; inv Ezs; simpl in *;
-        try discriminate.
-      + constructor; eapply Cofix; eauto.
-      + rewrite <-H, <-H4, <-H6.
-        constructor; eapply Cofix; eauto.
-      + rewrite <-H, <-H2, <-H6.
-        constructor; eapply Cofix; eauto.
-  Qed.
-
-  Add Parametric Morphism : ite
-      with signature @EqSt value ==> @EqSt value ==> @EqSt value ==> @EqSt value ==> Basics.impl
-        as ite_EqSt.
-  Proof.
-    cofix Cofix.
-    intros es es' Ees ts ts' Ets fs fs' Efs zs zs' Ezs H.
-    destruct es' as [[]], ts' as [[]], fs' as [[]], zs' as [[]];
-      inv H; inv Ees; inv Ets; inv Efs; inv Ezs; simpl in *;
-        try discriminate.
-      + constructor; eapply Cofix; eauto.
-      + rewrite <-H, <-H2, <-H6.
-        constructor; eapply Cofix; eauto.
-      + rewrite <-H, <-H4, <-H6.
-        constructor; eapply Cofix; eauto.
-  Qed.
-
-  Add Parametric Morphism k : (when k)
-      with signature @EqSt value ==> @EqSt value ==> @EqSt value ==> Basics.impl
-        as when_EqSt.
-  Proof.
-    cofix Cofix.
-    intros cs cs' Ecs xs xs' Exs ys ys' Eys H.
-    destruct cs' as [[]], xs' as [[]], ys' as [[]];
-      inv H; inv Ecs; inv Exs; inv Eys; simpl in *;
-        try discriminate.
-      + constructor; eapply Cofix; eauto.
-      + constructor.
-        * eapply Cofix; eauto.
-        * now inv H3.
-      + rewrite <-H, <-H5.
-        constructor.
-        * eapply Cofix; eauto.
-        * now inv H3.
-  Qed.
-
-  Add Parametric Morphism op t : (lift1 op t)
-      with signature @EqSt value ==> @EqSt value ==> Basics.impl
-        as lift1_EqSt.
-  Proof.
-    cofix Cofix.
-    intros es es' Ees ys ys' Eys Lift.
-    destruct es' as [[]], ys' as [[]];
-      inv Lift; inv Eys; inv Ees; simpl in *; try discriminate.
-    - constructor; eapply Cofix; eauto.
-    - constructor.
-      + now inv H1; inv H3.
-      + eapply Cofix; eauto.
-  Qed.
-
-  Add Parametric Morphism op t1 t2 : (lift2 op t1 t2)
-      with signature @EqSt value ==> @EqSt value ==> @EqSt value ==> Basics.impl
-        as lift2_EqSt.
-  Proof.
-    cofix Cofix.
-    intros e1s e1s' Ee1s e2s e2s' Ee2s ys ys' Eys Lift.
-    destruct e1s' as [[]], e2s' as [[]], ys' as [[]];
-      inv Lift; inv Eys; inv Ee1s; inv Ee2s; simpl in *; try discriminate.
-    - constructor; eapply Cofix; eauto.
-    - constructor.
-      + now inv H1; inv H3; inv H5.
-      + eapply Cofix; eauto.
-  Qed.
-
-  Add Parametric Morphism H : (sem_lexp H)
-      with signature @EqSt bool ==> eq ==> @EqSt value ==> Basics.impl
-        as sem_lexp_morph.
-  Proof.
-    intros ** b b' Eb e xs xs' Exs Sem.
-    revert b' xs' Eb Exs; induction Sem.
-    - intros. admit.
-    - econstructor; eauto.
-      eapply sem_var_EqSt; eauto.
-    - econstructor; eauto.
-      apply IHSem; auto; try reflexivity.
-      now rewrite <-Exs.
-    - econstructor.
-      + apply IHSem; auto; reflexivity.
-      + now rewrite <-Exs.
-    - econstructor.
-      + apply IHSem1; auto; reflexivity.
-      + apply IHSem2; auto; reflexivity.
-      + now rewrite <-Exs.
-  Qed.
-
-  Add Parametric Morphism H : (sem_cexp H)
-      with signature @EqSt bool ==> eq ==> @EqSt value ==> Basics.impl
-        as sem_cexp_morph.
-  Proof.
-    intros ** b b' Eb e xs xs' Exs Sem.
-    revert b' xs' Eb Exs; induction Sem.
-    - econstructor; eauto.
-      + apply IHSem1; auto; reflexivity.
-      + apply IHSem2; auto; reflexivity.
-      + now rewrite <-Exs.
-    - econstructor; eauto.
-      + rewrite <-Eb; eauto.
-      + apply IHSem1; auto; reflexivity.
-      + apply IHSem2; auto; reflexivity.
-      + now rewrite <-Exs.
-    - constructor.
-      now rewrite <-Eb, <-Exs.
-  Qed.
-
-  Add Parametric Morphism : Wire.merge_reset
-      with signature @EqSt bool ==> @EqSt bool ==> @EqSt bool
-        as merge_reset_EqSt.
-  Proof.
-    cofix Cofix.
-    intros r1 r1' Er1 r2 r2' Er2.
-    unfold_St r1; unfold_St r1'; unfold_St r2; unfold_St r2'.
-    constructor; inv Er1; inv Er2; simpl in *; auto.
-    now subst.
-  Qed.
-
-  CoFixpoint wire_fby1_EqSt_fix (v c: val)
-           (rs rs': Stream bool) (Ers: rs ≡ rs')
-           (xs xs': Stream value) (Exs: xs ≡ xs') :
-    Wire.fby1 rs v c xs ≡ Wire.fby1 rs' v c xs'
-  with wire_fby_EqSt_fix (c: val)
-                     (rs rs': Stream bool) (Ers: rs ≡ rs')
-                     (xs xs': Stream value) (Exs: xs ≡ xs') :
-         Wire.fby rs c xs ≡ Wire.fby rs' c xs'.
-  Proof.
-    - unfold_Stv rs; unfold_Stv rs'; unfold_Stv xs; unfold_Stv xs';
-        constructor; inv Exs; inv Ers; simpl in *; try discriminate; auto.
-      + inv H; apply wire_fby1_EqSt_fix; auto.
-      + inv H; apply wire_fby1_EqSt_fix; auto.
-    - unfold_Stv xs; unfold_Stv xs'; unfold_St rs; unfold_St rs';
-        constructor; inv Exs; inv Ers; simpl in *; try discriminate; auto.
-      inv H; apply wire_fby1_EqSt_fix; auto.
-  Qed.
-
-  Add Parametric Morphism : Wire.fby
-      with signature @EqSt bool ==> eq ==> @EqSt value ==> @EqSt value
-        as wire_fby_EqSt.
-  Proof. intros; apply wire_fby_EqSt_fix; auto. Qed.
-
-  Add Parametric Morphism : clocks_of
-      with signature @EqSts value ==> @EqSt bool
-        as clocks_of_EqSt.
-  Proof.
-    cofix Cofix.
-    intros xs xs' Exs.
-    constructor; simpl.
-    - clear Cofix.
-      revert dependent xs'.
-      induction xs; intros; try inv Exs; simpl; auto.
-      f_equal; auto.
-      now rewrite H1.
-    - apply Cofix.
-      clear Cofix.
-      revert dependent xs'.
-      induction xs; intros; try inv Exs; simpl; constructor.
-      + now rewrite H1.
-      + now apply IHxs.
-  Qed.
-
-  Fixpoint wire_sem_equation_morph_fix
-           (G: global) (H: history)
-           (b b': Stream bool) (Eb: b ≡ b')
-           (r r': Stream bool) (Er: r ≡ r')
-           (e: equation)
-           (Sem: Wire.sem_equation G H b r e) {struct Sem} :
-    Wire.sem_equation G H b' r' e
-  with wire_sem_node_morph_fix
-         (G: global)
-         (r r': Stream bool) (Er: r ≡ r')
-         (f: ident)
-         (xss xss': list (Stream value)) (Exss: EqSts value xss xss')
-         (yss yss': list (Stream value)) (Eyss: EqSts value yss yss')
-         (Sem: Wire.sem_node G r f xss yss) {struct Sem} :
-    Wire.sem_node G r' f xss' yss'.
-  Proof.
-    - induction Sem.
-      + econstructor; eauto.
-        now rewrite <-Eb.
-      + econstructor; eauto.
-        * apply Forall2_impl_In with (P:=sem_lexp H b); eauto.
-          intros; now rewrite <-Eb.
-        * eapply wire_sem_node_morph_fix; eauto; reflexivity.
-      + econstructor; eauto.
-        * apply Forall2_impl_In with (P:=sem_lexp H b); eauto.
-          intros; now rewrite <-Eb.
-        * eapply wire_sem_node_morph_fix; eauto; try reflexivity.
-          rewrite <-Er; reflexivity.
-      + econstructor; eauto.
-        * rewrite <-Eb; eauto.
-        * subst.
-          eapply sem_var_EqSt; eauto.
-          now rewrite <-Er.
-    - induction Sem.
-      econstructor; eauto.
-      + instantiate (1:=H).
-        now rewrite <-Exss.
-      + now rewrite <-Eyss.
-      + apply Forall_impl with (P:=Wire.sem_equation G H (clocks_of xss) r); auto.
-        apply wire_sem_equation_morph_fix; auto.
-        now rewrite Exss.
-  Admitted.
-
-  Add Parametric Morphism G H : (Wire.sem_equation G H)
-      with signature @EqSt bool ==> @EqSt bool ==> eq ==> Basics.impl
-        as wire_sem_equation_morph.
-  Proof.
-    unfold Basics.impl; apply wire_sem_equation_morph_fix.
-  Qed.
-
-  Add Parametric Morphism G : (Wire.sem_node G)
-      with signature @EqSt bool ==> eq ==> @EqSts value ==> @EqSts value ==> Basics.impl
-        as wire_sem_node_morph.
-  Proof.
-    unfold Basics.impl; apply wire_sem_node_morph_fix.
-  Qed.
-
-  Add Parametric Morphism c : (const c)
-      with signature @EqSt bool ==> @EqSt value
-        as const_EqSt.
-  Proof.
-    cofix; intros b b' Eb.
-    unfold_Stv b; unfold_Stv b';
-      constructor; inv Eb; simpl in *; try discriminate; auto.
-  Qed.
-
-  Add Parametric Morphism A opaque n : (Rec.mask opaque n)
-      with signature @EqSt bool ==> @EqSt A ==> @EqSt A
-        as mask_EqSt.
-  Proof.
-    revert n; cofix Cofix; intros n rs rs' Ers xs xs' Exs.
-    unfold_Stv rs; unfold_Stv rs'; unfold_St xs; unfold_St xs';
-      constructor; inv Ers; inv Exs;
-        simpl in *; try discriminate;
-          destruct n as [|[]]; auto; try reflexivity.
-  Qed.
+       (Mod          : NLSEMANTICSCOIND Ids Op OpAux Clks Syn Comm Ord).
 
   CoFixpoint false_s : Stream bool := false ::: false_s.
 
@@ -406,7 +41,7 @@ Module Type SEMEQUIV
 
     Remark fby1_equiv:
       forall c v xs,
-        Wire.fby1 false_s v (sem_const c) xs ≡ Rec.fby1 v (sem_const c) xs.
+        Wire.fby1 false_s v (sem_const c) xs ≡ Mod.fby1 v (sem_const c) xs.
     Proof.
       cofix; intros.
       unfold_Stv xs; constructor; simpl; auto.
@@ -414,7 +49,7 @@ Module Type SEMEQUIV
 
     Corollary fby_equiv:
       forall c xs,
-        Wire.fby false_s (sem_const c) xs ≡ Rec.fby (sem_const c) xs.
+        Wire.fby false_s (sem_const c) xs ≡ Mod.fby (sem_const c) xs.
     Proof.
       cofix; intros.
       unfold_Stv xs; constructor; simpl; auto.
@@ -466,7 +101,7 @@ Module Type SEMEQUIV
 
     (* Lemma flatten_masks_n_spec: *)
     (*   forall rs xs n, *)
-    (*     Rec.flatten_masks rs (Rec.masks_from n rs xs) ≡ xs. *)
+    (*     Mod.flatten_masks rs (Mod.masks_from n rs xs) ≡ xs. *)
     (* Proof. *)
     (*   cofix; intros. *)
     (*   unfold_Stv rs; unfold_St xs. *)
@@ -475,7 +110,7 @@ Module Type SEMEQUIV
 
     Lemma flatten_masks_spec:
       forall rs xs,
-        Rec.flatten_masks rs (Rec.masks rs xs) ≡ xs.
+        Mod.flatten_masks rs (Mod.masks rs xs) ≡ xs.
     Proof.
       cofix; intros.
       unfold_Stv rs; unfold_St xs.
@@ -501,12 +136,12 @@ Module Type SEMEQUIV
     Qed.
 
     Definition mask_history (n: nat) (rs: Stream bool) (H: history) : history :=
-      map_history (Rec.mask_v n rs) H.
+      map_history (Mod.mask_v n rs) H.
 
     Corollary mask_history_spec:
       forall n rs H x xs,
         sem_var H x xs ->
-        sem_var (mask_history n rs H) x (Rec.mask_v n rs xs).
+        sem_var (mask_history n rs H) x (Mod.mask_v n rs xs).
     Proof.
       intros; apply map_history_spec; auto.
       solve_proper.
@@ -515,7 +150,7 @@ Module Type SEMEQUIV
     Corollary mask_history_spec_Forall2:
       forall n rs H xs xss,
         Forall2 (sem_var H) xs xss ->
-        Forall2 (sem_var (mask_history n rs H)) xs (List.map (Rec.mask_v n rs) xss).
+        Forall2 (sem_var (mask_history n rs H)) xs (List.map (Mod.mask_v n rs) xss).
     Proof.
       intros.
       rewrite Forall2_map_2.
@@ -523,7 +158,7 @@ Module Type SEMEQUIV
       intros; apply mask_history_spec; auto.
     Qed.
 
-        Remark const_false_absent:
+    Remark const_false_absent:
       forall c,
         const c false_s ≡ Streams.const absent.
     Proof.
@@ -532,7 +167,7 @@ Module Type SEMEQUIV
 
     (* Remark mask_absent: *)
     (*   forall n rs, *)
-    (*     Rec.mask n rs (Streams.const absent) ≡ Streams.const absent. *)
+    (*     Mod.mask n rs (Streams.const absent) ≡ Streams.const absent. *)
     (* Proof. *)
     (*   cofix; intros. *)
     (*   unfold_Stv rs; constructor; destruct n as [|[]]; *)
@@ -550,7 +185,7 @@ Module Type SEMEQUIV
 
     Remark mask_sem_const:
       forall n rs c b,
-        Rec.mask_v n rs (const c b) ≡ const c (Rec.mask_b n rs b).
+        Mod.mask_v n rs (const c b) ≡ const c (Mod.mask_b n rs b).
     Proof.
       cofix; intros.
       unfold_Stv rs; unfold_Stv b; destruct n as [|[]];
@@ -569,12 +204,12 @@ Module Type SEMEQUIV
     Corollary when_mask:
       forall n rs k es xs os,
         when k es xs os ->
-        when k (Rec.mask_v n rs es) (Rec.mask_v n rs xs) (Rec.mask_v n rs os).
+        when k (Mod.mask_v n rs es) (Mod.mask_v n rs xs) (Mod.mask_v n rs os).
     Proof.
       cofix; intros.
-      rewrite (unfold_Stream (Rec.mask_v n rs es));
-        rewrite (unfold_Stream (Rec.mask_v n rs xs));
-        rewrite (unfold_Stream (Rec.mask_v n rs os)).
+      rewrite (unfold_Stream (Mod.mask_v n rs es));
+        rewrite (unfold_Stream (Mod.mask_v n rs xs));
+        rewrite (unfold_Stream (Mod.mask_v n rs os)).
       unfold_Stv rs; unfold_Stv es; unfold_St xs; unfold_St os;
         destruct n as [|[]]; try (now inv H; constructor; auto).
       rewrite <-unfold_Stream; apply when_absent.
@@ -592,11 +227,11 @@ Module Type SEMEQUIV
     Corollary lift1_mask:
       forall n rs op t es os,
         lift1 op t es os ->
-        lift1 op t (Rec.mask_v n rs es) (Rec.mask_v n rs os).
+        lift1 op t (Mod.mask_v n rs es) (Mod.mask_v n rs os).
     Proof.
       cofix; intros.
-      rewrite (unfold_Stream (Rec.mask_v n rs es));
-        rewrite (unfold_Stream (Rec.mask_v n rs os)).
+      rewrite (unfold_Stream (Mod.mask_v n rs es));
+        rewrite (unfold_Stream (Mod.mask_v n rs os)).
       unfold_Stv rs; unfold_Stv es; unfold_St os;
         destruct n as [|[]]; try (now inv H; constructor; auto).
       rewrite <-unfold_Stream; apply lift1_absent.
@@ -614,12 +249,12 @@ Module Type SEMEQUIV
     Corollary lift2_mask:
       forall n rs op t1 t2 e1s e2s os,
         lift2 op t1 t2 e1s e2s os ->
-        lift2 op t1 t2 (Rec.mask_v n rs e1s) (Rec.mask_v n rs e2s) (Rec.mask_v n rs os).
+        lift2 op t1 t2 (Mod.mask_v n rs e1s) (Mod.mask_v n rs e2s) (Mod.mask_v n rs os).
     Proof.
       cofix; intros.
-      rewrite (unfold_Stream (Rec.mask_v n rs e1s));
-        rewrite (unfold_Stream (Rec.mask_v n rs e2s));
-        rewrite (unfold_Stream (Rec.mask_v n rs os)).
+      rewrite (unfold_Stream (Mod.mask_v n rs e1s));
+        rewrite (unfold_Stream (Mod.mask_v n rs e2s));
+        rewrite (unfold_Stream (Mod.mask_v n rs os)).
       unfold_Stv rs; unfold_Stv e1s; unfold_Stv e2s; unfold_St os;
         destruct n as [|[]]; try (now inv H; constructor; auto).
       rewrite <-unfold_Stream; apply lift2_absent.
@@ -629,10 +264,10 @@ Module Type SEMEQUIV
     Lemma mask_sem_lexp:
       forall n rs H b e es,
         sem_lexp H b e es ->
-        sem_lexp (mask_history n rs H) (Rec.mask_b n rs b) e (Rec.mask_v n rs es).
+        sem_lexp (mask_history n rs H) (Mod.mask_b n rs b) e (Mod.mask_v n rs es).
     Proof.
       intros ** Sem; induction Sem.
-      - rewrite mask_sem_const; constructor.
+      - constructor; rewrite H0; apply mask_sem_const.
       - constructor; apply mask_history_spec; auto.
       - econstructor; eauto.
         + apply mask_history_spec; eauto.
@@ -654,13 +289,13 @@ Module Type SEMEQUIV
     Corollary merge_mask:
       forall n rs xs ts fs os,
         merge xs ts fs os ->
-        merge (Rec.mask_v n rs xs) (Rec.mask_v n rs ts) (Rec.mask_v n rs fs) (Rec.mask_v n rs os).
+        merge (Mod.mask_v n rs xs) (Mod.mask_v n rs ts) (Mod.mask_v n rs fs) (Mod.mask_v n rs os).
     Proof.
       cofix; intros.
-      rewrite (unfold_Stream (Rec.mask_v n rs xs));
-        rewrite (unfold_Stream (Rec.mask_v n rs ts));
-        rewrite (unfold_Stream (Rec.mask_v n rs fs));
-        rewrite (unfold_Stream (Rec.mask_v n rs os)).
+      rewrite (unfold_Stream (Mod.mask_v n rs xs));
+        rewrite (unfold_Stream (Mod.mask_v n rs ts));
+        rewrite (unfold_Stream (Mod.mask_v n rs fs));
+        rewrite (unfold_Stream (Mod.mask_v n rs os)).
       unfold_Stv rs; unfold_St xs; unfold_St ts; unfold_St fs; unfold_St os;
         destruct n as [|[]]; try (now inv H; constructor; auto).
       rewrite <-unfold_Stream; apply merge_absent.
@@ -677,13 +312,13 @@ Module Type SEMEQUIV
     Corollary ite_mask:
       forall n rs es ts fs os,
         ite es ts fs os ->
-        ite (Rec.mask_v n rs es) (Rec.mask_v n rs ts) (Rec.mask_v n rs fs) (Rec.mask_v n rs os).
+        ite (Mod.mask_v n rs es) (Mod.mask_v n rs ts) (Mod.mask_v n rs fs) (Mod.mask_v n rs os).
     Proof.
       cofix; intros.
-      rewrite (unfold_Stream (Rec.mask_v n rs es));
-        rewrite (unfold_Stream (Rec.mask_v n rs ts));
-        rewrite (unfold_Stream (Rec.mask_v n rs fs));
-        rewrite (unfold_Stream (Rec.mask_v n rs os)).
+      rewrite (unfold_Stream (Mod.mask_v n rs es));
+        rewrite (unfold_Stream (Mod.mask_v n rs ts));
+        rewrite (unfold_Stream (Mod.mask_v n rs fs));
+        rewrite (unfold_Stream (Mod.mask_v n rs os)).
       unfold_Stv rs; unfold_St es; unfold_St ts; unfold_St fs; unfold_St os;
         destruct n as [|[]]; try (now inv H; constructor; auto).
       rewrite <-unfold_Stream; apply ite_absent.
@@ -692,7 +327,7 @@ Module Type SEMEQUIV
     Lemma mask_sem_cexp:
       forall n rs H b e es,
         sem_cexp H b e es ->
-        sem_cexp (mask_history n rs H) (Rec.mask_b n rs b) e (Rec.mask_v n rs es).
+        sem_cexp (mask_history n rs H) (Mod.mask_b n rs b) e (Mod.mask_v n rs es).
     Proof.
       intros ** Sem; induction Sem.
       - econstructor; eauto.
@@ -704,52 +339,185 @@ Module Type SEMEQUIV
       - constructor; apply mask_sem_lexp; auto.
     Qed.
 
-    Lemma WireRec_node_reset:
-      forall rs f ess oss,
-        Wire.sem_node G (Wire.merge_reset false_s (reset_of rs)) f ess oss ->
-        (* Rec.sem_node G f ess oss -> *)
-        Rec.sem_reset G f (reset_of rs) ess oss.
+    Remark fby_absent:
+      forall c, Mod.fby c (Streams.const absent) ≡ Streams.const absent.
     Proof.
-      intros ** Reset (* Node *).
-      rewrite merge_reset_with_false in Reset.
-      constructor.
-      inversion_clear Reset as [? ? ? ? ? ? ? In Out Sem].
-      intro i.
-      econstructor; eauto.
-      instantiate (1:=mask_history i (reset_of rs) H).
-      - now apply mask_history_spec_Forall2.
-      - now apply mask_history_spec_Forall2.
-      - induction (n_eqs n) as [|e]; auto.
-        inversion_clear Sem as [|? ? Sem_e].
-        constructor; auto.
-        remember (clocks_of ess) as b.
-        remember (reset_of rs) as r.
-        induction Sem_e as [? ? ? ? ? ? ? Sem Sem_var| | |].
-        + apply (mask_history_spec i r) in Sem_var.
-          econstructor; eauto.
+      cofix; intro.
+      rewrite (unfold_Stream (Streams.const absent)); constructor; simpl; auto.
+    Qed.
 
-      - econstructor; eauto.
-      - econstructor. clear; induction xss.
-        + eexists; eauto.
+    Remark fby1_absent:
+      forall v c, Mod.fby1 v c (Streams.const absent) ≡ Streams.const absent.
+    Proof.
+      cofix; intro.
+      rewrite (unfold_Stream (Streams.const absent)); constructor; simpl; auto.
+    Qed.
 
+    (* Remark foo: *)
+    (*   forall n rs c0 c xs, *)
+    (*     Mod.mask absent n rs (Wire.fby1 rs c0 c xs) ≡ Mod.fby1 c0 c (Mod.mask absent n rs xs). *)
+    (* Proof. *)
+    (*   cofix Cofix; intros. *)
+    (*   unfold_Stv rs; unfold_Stv xs; *)
+    (*     constructor; destruct n as [|[]]; simpl; fold Wire.fby; auto. *)
+    (*     + rewrite fby1_absent; reflexivity. *)
+    (*     + rewrite fby1_absent; reflexivity. *)
+    (*   - cofix Cofix; intros. *)
+    (*     unfold_Stv rs; unfold_Stv xs; constructor; destruct n; *)
+    (*       simpl; fold Wire.fby; auto. *)
+    (*     destruct n. *)
+    (*     simpl. *)
+    (*     fold Wire.fby.  *)
+    (*     simpl. auto. *)
+    (*     simpl. auto. *)
+    (*       constructor; simpl; auto. *)
+
+    (*     rewrite <-Cofix. unfold Wire.fby1. reflexivity. *)
+    Remark mask_fby:
+      forall n rs c xs,
+        Mod.mask_v n rs (Wire.fby rs c xs) ≡ Mod.fby c (Mod.mask_v n rs xs).
+    Proof.
+      cofix Cofix; intros.
+      unfold_Stv rs; unfold_Stv xs; destruct n as [|[]];
+        constructor; simpl; auto.
+      - rewrite fby_absent; reflexivity.
+      - rewrite fby_absent; reflexivity.
+      - admit.
+      - admit.
+      - admit.
+      - admit.
+      - admit.
     Admitted.
 
-    Lemma WireRec_equation_node:
+    Remark clocks_of_nil_absent:
+      clocks_of [] ≡ Streams.const false.
+    Proof.
+      cofix.
+      rewrite unfold_Stream; rewrite (unfold_Stream (clocks_of [])).
+      constructor; simpl; auto.
+    Qed.
+
+    (* Remark clocks_of_absent: *)
+    (*   clocks_of  *)
+    Remark mask_clocks_of:
+      forall n rs xss,
+        Mod.mask_b n rs (clocks_of xss) ≡ clocks_of (List.map (Mod.mask_v n rs) xss).
+    Proof.
+      cofix; intros.
+      induction xss as [|xs]; simpl.
+      - unfold_Stv rs; rewrite (unfold_Stream (clocks_of []));
+          constructor; destruct n as [|[]]; simpl; auto;
+            rewrite clocks_of_nil_absent; try apply Mod.mask_const_opaque.
+        reflexivity.
+      - unfold_Stv rs; unfold_Stv xs;
+          constructor; destruct n as [|[]]; simpl; auto;
+            try match goal with
+                  |- _ = _ => clear; induction xss as [|[]]; simpl; auto
+                end.
+        + clear; induction xss as [|[[]]]; simpl; auto.
+        + admit.
+        + admit.
+        + admit.
+        + admit.
+        + admit.
+        + admit.
+        + clear; induction xss as [|[[]]]; simpl; auto.
+        + admit.
+        + admit.
+        + admit.
+        + admit.
+        + admit.
+        + admit.
+    Admitted.
+
+    Remark reset_of_absent:
+      reset_of (Streams.const absent) ≡ Streams.const false.
+    Proof.
+      cofix.
+      rewrite unfold_Stream; rewrite (unfold_Stream (Streams.const absent)).
+      constructor; simpl; auto.
+    Qed.
+
+    Remark mask_reset_of:
+      forall n rs xs,
+        reset_of (Mod.mask_v n rs xs) ≡ Mod.mask_b n rs (reset_of xs).
+    Proof.
+      cofix; intros.
+      unfold_Stv rs; unfold_Stv xs;
+        constructor; destruct n as [|[]]; simpl; auto;
+          apply reset_of_absent.
+    Qed.
+
+    Lemma WireMod_node_reset:
+      forall rs f ess oss,
+        Wire.sem_node G (reset_of rs) f ess oss ->
+        Mod.sem_reset G f (reset_of rs) ess oss.
+    Proof.
+      intros ** Reset.
+      constructor.
+      induction Reset
+        as [? ? ? ? ? ? ? ? Sem_var
+              |? ? ? ? ? ? ? ? ? ? ? Sem_vars
+              |? ? ? ? ? ? ? ? ? ? ? ? ? Sem_var Sem_vars
+              |? ? ? ? ? ? ? ? ? ? ? Sem_var |]
+             using Wire.sem_node_mult with
+          (P_equation := fun H b r e =>
+                           forall i,
+                             Wire.sem_equation G H b r e ->
+                             Mod.sem_equation G (mask_history i r H) (Mod.mask_b i r b) e);
+        intros.
+      - apply (mask_history_spec i r) in Sem_var.
+        econstructor; eauto.
+        now apply mask_sem_cexp.
+      - apply (mask_history_spec_Forall2 i r) in Sem_vars.
+        econstructor; eauto.
+        eapply Forall2_map_2, Forall2_impl_In; eauto.
+        intros; now apply mask_sem_lexp.
+      - apply (mask_history_spec i r) in Sem_var.
+        apply (mask_history_spec_Forall2 i r) in Sem_vars.
+        econstructor; eauto.
+        instantiate (1 := List.map (Mod.mask_v i r) ess).
+        + eapply Forall2_map_2, Forall2_impl_In; eauto.
+          intros; apply mask_sem_lexp; auto.
+        + rewrite mask_reset_of.
+          constructor.
+          intro n; specialize (IHReset n).
+          eapply Mod.mod_sem_node_morph; eauto.
+          * rewrite List.map_map.
+            apply map_EqSt; try reflexivity. admit.
+      - apply (mask_history_spec i r) in Sem_var.
+        econstructor; eauto.
+        + eapply mask_sem_lexp; eauto.
+        + inv Sem_var.
+          econstructor; eauto.
+          now rewrite <-mask_fby.
+      - econstructor; eauto.
+        instantiate (1:=mask_history n0 r H).
+        + now apply mask_history_spec_Forall2.
+        + now apply mask_history_spec_Forall2.
+        + induction (n_eqs n) as [|e]; auto.
+          inversion_clear H3 as [|? ? Sem_e].
+          inversion_clear H4.
+          constructor; auto.
+          rewrite <-mask_clocks_of; auto.
+    Qed.
+
+    Lemma WireMod_equation_node:
       (forall H b r e,
           Wire.sem_equation G H b r e ->
           (* r = false_s -> *)
-          Rec.sem_equation G H b e)
+          Mod.sem_equation G H b e)
       /\
       (forall r f xss oss,
           Wire.sem_node G r f xss oss ->
-          Rec.sem_node G f xss oss).
+          Mod.sem_node G f xss oss).
     Proof.
       Check Wire.sem_equation_node_ind.
       apply Wire.sem_equation_node_ind; intros.
       - econstructor; eauto.
       - econstructor; eauto.
       - econstructor; eauto.
-        eapply WireRec_node_reset; eauto.
+        eapply WireMod_node_reset; eauto.
       - econstructor; eauto.
         subst; now apply fby_equiv.
       - econstructor; eauto.
@@ -757,14 +525,14 @@ Module Type SEMEQUIV
         auto.
     Qed.
 
-    Theorem WireRec:
+    Theorem WireMod:
       forall G f xss yss,
         Wire.sem_node G false_s f xss yss
-        <-> Rec.sem_node G f xss yss.
+        <-> Mod.sem_node G f xss yss.
     Proof.
       split; intro Sem; inv Sem; econstructor; eauto; eapply Forall_impl;
-        [ now apply WireRec_equation | auto
-          | now apply WireRec_equation | auto ].
+        [ now apply WireMod_equation | auto
+          | now apply WireMod_equation | auto ].
     Qed.
 
     SearchAbout Forall.
